Pset2 exp done

pset02_BinomialCoefficients/Pset2.v
@@ -135,14 +135,36 @@ Module Impl.
   (* Exercise: Define a simple exponentiation function in the same style, so that
      "exp base n" equals "base^n". *)
 
-  Definition exp(base: N): N -> N. Admitted.
+  Definition exp(base: N): N -> N :=
+    recurse by cases
+    | 0 => 1
+    | n + 1 => base * recurse
+    end. 
 
   (* Once you define "exp", you can replace "Admitted." below by "Proof. equality. Qed." *)
-  Lemma test_exp_2_3: exp 2 3 = 8. Admitted.
-  Lemma test_exp_3_2: exp 3 2 = 9. Admitted.
-  Lemma test_exp_4_1: exp 4 1 = 4. Admitted.
-  Lemma test_exp_5_0: exp 5 0 = 1. Admitted.
-  Lemma test_exp_1_3: exp 1 3 = 1. Admitted.
+  Lemma test_exp_2_3: exp 2 3 = 8.
+  Proof. 
+    simpl. equality. 
+  Qed.
+  Lemma test_exp_3_2: exp 3 2 = 9.
+  Proof. 
+    simpl. equality. 
+  Qed.
+  
+  Lemma test_exp_4_1: exp 4 1 = 4.
+  Proof. 
+    simpl. equality. 
+  Qed.
+ 
+  Lemma test_exp_5_0: exp 5 0 = 1.
+  Proof. 
+    simpl. equality. 
+  Qed.
+
+  Lemma test_exp_1_3: exp 1 3 = 1.
+  Proof. 
+    simpl. equality. 
+  Qed.
 
   (* Here's another recursive function defined in the same style to apply a
      function f to a range of values:
